Got ml_translatorScript working with modules.
I didn't get evaluate_decs'_empty_store_IMP and
evaluate_decs'_empty_store working, but they don't appear to be used
anywhere.

ml_optimiseScript fails now.

print_ast/Print_astTerminationScript.sml
@@ -51,7 +51,7 @@ val (exp_to_tok_tree_def, exp_to_tok_tree_ind) =
   TRY (induct_on `funs`) >>
   TRY (induct_on `pes`) >>
   TRY (induct_on `es`) >>
-  TRY (induct_on `v50`) >>
+  TRY (induct_on `v51`) >>
   rw [exp_size_def] >>
   fs [exp_size_def] >>
   rw [exp_size_def] >>
@@ -64,7 +64,9 @@ val (type_to_tok_tree_def, type_to_tok_tree_ind) =
   wf_rel_tac `measure t_size` >>
   srw_tac [ARITH_ss] [] >>
   srw_tac [ARITH_ss] [] >>
-  induct_on `v14` >>
+  TRY (qpat_assum `ts ≠ []` (fn _ => all_tac)) >>
+  TRY (induct_on `v16`) >>
+  TRY (induct_on `ts`) >>
   rw [] >>
   fs [t_size_def] >>
   res_tac >>
